src/test/RIoT.Test.Definitions.fst
@@ -19,31 +19,28 @@ open ASN1.Spec
 open ASN1.Low
 open X509
 
-// open RIoT.X509
 open RIoT.Base
-// open RIoT.Declassify
-// open RIoT.Helpers
+open RIoT.X509.Base
+open RIoT.Declassify
+open RIoT.Helpers
 // open RIoT.Spec
 // open RIoT.Impl
 // open RIoT.Core
 
 module Ed25519 = Hacl.Ed25519
 
-#set-options "--z3rlimit 64 --fuel 4 --ifuel 0"
+#set-options "--z3rlimit 64 --fuel 4 --ifuel 0 --using_facts_from '* -FStar.Tactics -FStar.Reflection'"
 
 let aliasKeyCrt_version: x509_version_t = normalize_term x509_version_3
 
 (* AliasKeyTBS SerialNumber *)
 let aliasKeyCrt_serialNumber_len = 2ul
 noextract inline_for_extraction let aliasKeyCrt_serialNumber_list
-: List.llist byte_pub (v aliasKeyCrt_serialNumber_len)
+: l: List.llist byte_pub (v aliasKeyCrt_serialNumber_len)
+  { valid_big_integer_as_octet_string aliasKeyCrt_serialNumber_len (B32.hide (Seq.createL l)) /\
+    filter_x509_serialNumber (asn1_get_big_integer_as_octet_string aliasKeyCrt_serialNumber_len (B32.hide (Seq.createL l))) }
 = [0x01uy; 0x03uy]
 let aliasKeyCrt_serialNumber_buf = IB.igcmalloc_of_list HS.root aliasKeyCrt_serialNumber_list
-
-// let aliasKeyCrt_serialNumber: x509_serialNumber_t
-// = normalize_term ([@inline_let] let x: big_integer_as_octet_string_t = (|1ul, B32.create 1ul 1uy|) in
-//   assert_norm (filter_x509_serialNumber x);
-//   x)
 
 (* AliasKeyTBS Names *)
 let aliasKeyCrt_s_common_len = 2ul
@@ -82,20 +79,182 @@ noextract inline_for_extraction let aliasKeyCrt_i_country_list
 = [0x41uy; 0x42uy]
 let aliasKeyCrt_i_country_buf = IB.igcmalloc_of_list HS.root aliasKeyCrt_i_country_list
 
-// let s_common: x509_RDN_x520_attribute_string_t COMMON_NAME IA5_STRING
-// = normalize_term (asn1_get_character_string #IA5_STRING 2ul (B32.create 2ul 1uy))
+(* DeviceID CSR *)
+let deviceIDCSR_s_common_len = 2ul
+noextract inline_for_extraction let deviceIDCSR_s_common_list
+: character_string_llist IA5_STRING deviceIDCSR_s_common_len
+= [0x01uy; 0x03uy]
+let deviceIDCSR_s_common_buf = IB.igcmalloc_of_list HS.root deviceIDCSR_s_common_list
 
-// let s_org: x509_RDN_x520_attribute_string_t ORGANIZATION IA5_STRING
-// = normalize_term (asn1_get_character_string #IA5_STRING 2ul (B32.create 2ul 0uy))
+let deviceIDCSR_s_org_len = 2ul
+noextract inline_for_extraction let deviceIDCSR_s_org_list
+: character_string_llist IA5_STRING deviceIDCSR_s_org_len
+= [0x01uy; 0x03uy]
+let deviceIDCSR_s_org_buf = IB.igcmalloc_of_list HS.root deviceIDCSR_s_org_list
 
-// let s_country: x509_RDN_x520_attribute_string_t COMMON_NAME PRINTABLE_STRING
-// = normalize_term (asn1_get_character_string #PRINTABLE_STRING 2ul (B32.create 2ul 0x41uy))
+let deviceIDCSR_s_country_len = 2ul
+noextract inline_for_extraction let deviceIDCSR_s_country_list
+: character_string_llist PRINTABLE_STRING deviceIDCSR_s_country_len
+= [0x41uy; 0x42uy]
+let deviceIDCSR_s_country_buf = IB.igcmalloc_of_list HS.root deviceIDCSR_s_country_list
 
-// let notBefore: datatype_of_asn1_type Generalized_Time
-// = x509_validity_notAfter_default
+unfold inline_for_extraction
+let deviceIDCSR_keyUsage = normalize_term aliasKeyCrt_key_usage
 
-// let notAfter: datatype_of_asn1_type Generalized_Time
-// = x509_validity_notAfter_default
+#set-options "--z3rlimit 64 --fuel 0 --ifuel 0"
+inline_for_extraction
+let riot_get_deviceIDCSR_ingredients ()
+: HST.Stack deviceIDCSR_ingredients_t
+  (requires fun h -> True)
+  (ensures fun h0 _ h1 -> B.modifies B.loc_none h0 h1)
+= let ku: key_usage_payload_t = deviceIDCSR_keyUsage in
 
-// let aliasKeyCrt_keyID: datatype_of_asn1_type OCTET_STRING
-// = normalize_term (|1ul, B32.create 1ul 1uy|)
+  let deviceIDCSR_version: x509_version_t = x509_version_3 in
+
+  IB.recall deviceIDCSR_s_common_buf;
+  IB.recall_contents deviceIDCSR_s_common_buf (Seq.createL deviceIDCSR_s_common_list);
+  let deviceIDCSR_s_common: x509_RDN_x520_attribute_string_t COMMON_NAME IA5_STRING =
+    normalize_term ( asn1_get_character_string
+                       #IA5_STRING
+                       deviceIDCSR_s_common_len
+                       (B32.of_buffer deviceIDCSR_s_common_len deviceIDCSR_s_common_buf) ) in
+
+  IB.recall deviceIDCSR_s_org_buf;
+  IB.recall_contents deviceIDCSR_s_org_buf (Seq.createL deviceIDCSR_s_org_list);
+  let deviceIDCSR_s_org: x509_RDN_x520_attribute_string_t ORGANIZATION IA5_STRING =
+    normalize_term ( asn1_get_character_string
+                       #IA5_STRING
+                       deviceIDCSR_s_org_len
+                       (B32.of_buffer deviceIDCSR_s_org_len deviceIDCSR_s_org_buf) ) in
+
+  IB.recall deviceIDCSR_s_country_buf;
+  IB.recall_contents deviceIDCSR_s_country_buf (Seq.createL deviceIDCSR_s_country_list);
+  let deviceIDCSR_s_country: x509_RDN_x520_attribute_string_t COUNTRY PRINTABLE_STRING =
+    normalize_term ( asn1_get_character_string
+                       #PRINTABLE_STRING
+                       deviceIDCSR_s_country_len
+                       (B32.of_buffer deviceIDCSR_s_country_len deviceIDCSR_s_country_buf) ) in
+
+  let deviceIDCSR_ingredients: deviceIDCSR_ingredients_t = {
+    deviceIDCSR_ku        = ku;
+    deviceIDCSR_version   = deviceIDCSR_version;
+    deviceIDCSR_s_common  = deviceIDCSR_s_common;
+    deviceIDCSR_s_org     = deviceIDCSR_s_org;
+    deviceIDCSR_s_country = deviceIDCSR_s_country
+  } in
+
+  deviceIDCSR_ingredients
+
+inline_for_extraction
+let riot_get_aliasKeyCRT_ingredients ()
+: HST.Stack aliasKeyCRT_ingredients_t
+  (requires fun h -> True)
+  (ensures fun h0 _ h1 -> B.modifies B.loc_none h0 h1)
+= let ku: key_usage_payload_t = deviceIDCSR_keyUsage in
+
+  let riot_version: datatype_of_asn1_type INTEGER = 1l in
+
+  IB.recall aliasKeyCrt_serialNumber_buf;
+  IB.recall_contents aliasKeyCrt_serialNumber_buf (Seq.createL aliasKeyCrt_serialNumber_list);
+  let aliasKeyCrt_serialNumber: x509_serialNumber_t =
+    x509_get_serialNumber
+      (aliasKeyCrt_serialNumber_len)
+      (B32.of_buffer aliasKeyCrt_serialNumber_len aliasKeyCrt_serialNumber_buf) in
+
+  comment "AliasKey Crt Subject Names";
+  IB.recall aliasKeyCrt_s_common_buf;
+  IB.recall_contents aliasKeyCrt_s_common_buf (Seq.createL aliasKeyCrt_s_common_list);
+  let aliasKeyCrt_s_common: x509_RDN_x520_attribute_string_t COMMON_NAME IA5_STRING =
+    normalize_term ( asn1_get_character_string
+                       #IA5_STRING
+                       aliasKeyCrt_s_common_len
+                       (B32.of_buffer aliasKeyCrt_s_common_len aliasKeyCrt_s_common_buf) ) in
+
+  IB.recall aliasKeyCrt_s_org_buf;
+  IB.recall_contents aliasKeyCrt_s_org_buf (Seq.createL aliasKeyCrt_s_org_list);
+  let aliasKeyCrt_s_org: x509_RDN_x520_attribute_string_t ORGANIZATION IA5_STRING =
+    normalize_term ( asn1_get_character_string
+                       #IA5_STRING
+                       aliasKeyCrt_s_org_len
+                       (B32.of_buffer aliasKeyCrt_s_org_len aliasKeyCrt_s_org_buf) ) in
+
+  IB.recall aliasKeyCrt_s_country_buf;
+  IB.recall_contents aliasKeyCrt_s_country_buf (Seq.createL aliasKeyCrt_s_country_list);
+  let aliasKeyCrt_s_country: x509_RDN_x520_attribute_string_t COUNTRY PRINTABLE_STRING =
+    normalize_term ( asn1_get_character_string
+                       #PRINTABLE_STRING
+                       aliasKeyCrt_s_country_len
+                       (B32.of_buffer aliasKeyCrt_s_country_len aliasKeyCrt_s_country_buf) ) in
+
+  comment "AliasKey Crt Issuer Names";
+  IB.recall aliasKeyCrt_i_common_buf;
+  IB.recall_contents aliasKeyCrt_i_common_buf (Seq.createL aliasKeyCrt_i_common_list);
+  let aliasKeyCrt_i_common: x509_RDN_x520_attribute_string_t COMMON_NAME IA5_STRING =
+    normalize_term ( asn1_get_character_string
+                       #IA5_STRING
+                       aliasKeyCrt_i_common_len
+                       (B32.of_buffer aliasKeyCrt_i_common_len aliasKeyCrt_i_common_buf) ) in
+
+  IB.recall aliasKeyCrt_i_org_buf;
+  IB.recall_contents aliasKeyCrt_i_org_buf (Seq.createL aliasKeyCrt_i_org_list);
+  let aliasKeyCrt_i_org: x509_RDN_x520_attribute_string_t ORGANIZATION IA5_STRING =
+    normalize_term ( asn1_get_character_string
+                       #IA5_STRING
+                       aliasKeyCrt_i_org_len
+                       (B32.of_buffer aliasKeyCrt_i_org_len aliasKeyCrt_i_org_buf) ) in
+
+  IB.recall aliasKeyCrt_i_country_buf;
+  IB.recall_contents aliasKeyCrt_i_country_buf (Seq.createL aliasKeyCrt_i_country_list);
+  let aliasKeyCrt_i_country: x509_RDN_x520_attribute_string_t COUNTRY PRINTABLE_STRING =
+    normalize_term ( asn1_get_character_string
+                       #PRINTABLE_STRING
+                       aliasKeyCrt_i_country_len
+                       (B32.of_buffer aliasKeyCrt_i_country_len aliasKeyCrt_i_country_buf) ) in
+
+  IB.recall x509_validity_notAfter_default_buffer;
+  IB.recall_contents x509_validity_notAfter_default_buffer asn1_generalized_time_for_x509_validity_notAfter_default_seq;
+  let notBefore: datatype_of_asn1_type Generalized_Time = B32.of_buffer 15ul x509_validity_notAfter_default_buffer in
+  let notAfter : datatype_of_asn1_type Generalized_Time = B32.of_buffer 15ul x509_validity_notAfter_default_buffer in
+
+  let aliasKeyCRT_ingredients: aliasKeyCRT_ingredients_t = {
+    aliasKeyCrt_version      = aliasKeyCrt_version;
+    aliasKeyCrt_serialNumber = aliasKeyCrt_serialNumber;
+    aliasKeyCrt_i_common     = aliasKeyCrt_i_common;
+    aliasKeyCrt_i_org        = aliasKeyCrt_i_org;
+    aliasKeyCrt_i_country    = aliasKeyCrt_i_country;
+    aliasKeyCrt_notBefore    = notBefore;
+    aliasKeyCrt_notAfter     = notAfter;
+    aliasKeyCrt_s_common     = aliasKeyCrt_s_common;
+    aliasKeyCrt_s_org        = aliasKeyCrt_s_org;
+    aliasKeyCrt_s_country    = aliasKeyCrt_s_country;
+    aliasKeyCrt_ku           = ku;
+    aliasKeyCrt_riot_version = riot_version
+  } in
+
+  aliasKeyCRT_ingredients
+
+[@@ "opaque_to_smt"]
+inline_for_extraction
+let dump_riot
+  (deviceID_pub : B.lbuffer byte_pub 32)
+  (aliasKey_pub : B.lbuffer byte_pub 32)
+  (aliasKey_priv: B.lbuffer byte_sec 32)
+  (deviceIDCSR_len: UInt32.t)
+  (deviceIDCSR_buf: B.lbuffer byte_pub (v deviceIDCSR_len))
+  (aliasKeyCRT_len: UInt32.t)
+  (aliasKeyCRT_buf: B.lbuffer byte_pub (v aliasKeyCRT_len))
+: HST.Stack unit
+  (requires fun h ->
+    B.all_live h [B.buf deviceID_pub; B.buf aliasKey_pub; B.buf aliasKey_priv; B.buf deviceIDCSR_buf; B.buf aliasKeyCRT_buf])
+  (ensures fun h0 _ h1 ->
+    B.modifies B.loc_none h0 h1)
+= HST.push_frame ();
+  let aliasKey_priv_pub: B.lbuffer byte_pub 32 = B.alloca 0x00uy 32ul in
+  declassify_secret_buffer 32ul aliasKey_priv aliasKey_priv_pub;
+
+  write_out "DeviceIDPublicKey.hex"  aliasKey_pub 32ul;
+  write_out "AliasKeyPublicKey.hex"  aliasKey_pub 32ul;
+  write_out "AliasKeyPrivateKey.hex" aliasKey_priv_pub 32ul;
+  write_out "DeviceIDCSR.hex" deviceIDCSR_buf deviceIDCSR_len;
+  write_out "AliasKeyCrt.hex" aliasKeyCRT_buf aliasKeyCRT_len;
+  HST.pop_frame ()
